finished *lambda*-f

TypedAssembly/LambdaF/Term.lean
@@ -1,4 +1,4 @@
-import «TypedAssembly».LambdaF.Typ
+import «TypedAssembly».LambdaF.TypF
 import «TypedAssembly».Common.Prim
 import «TypedAssembly».LambdaF.TermEnv
 
@@ -6,21 +6,21 @@ inductive Term : {Δ : Ctxt} → Ctx Δ → Δ ⊢F⋆ ⋆ → Type where
   | int  {Γ : Ctx Δ} : Int → Term Γ .int
   | var  {Γ : Ctx Δ} {t : Δ ⊢F⋆ ⋆} : Γ ∋ t → Term Γ t
 
-  | fix  {Γ : Ctx Δ} {t₁ t₂ : Δ ⊢F⋆ ⋆} : Term (Γ ,, ⋆⟪ !t₁ → !t₂ ⟫ ,, t₁ ) t₂ → Term Γ ⋆⟪ !t₁ → !t₂ ⟫
-  | app  {Γ : Ctx Δ} {t₁ t₂ : Δ ⊢F⋆ ⋆} : Term Γ ⋆⟪ !t₁ → !t₂ ⟫ → Term Γ t₁ → Term Γ t₂
+  | fix  {Γ : Ctx Δ} {t₁ t₂ : Δ ⊢F⋆ ⋆} : Term (Γ ,, f⋆⟪ !t₁ → !t₂ ⟫ ,, t₁ ) t₂ → Term Γ f⋆⟪ !t₁ → !t₂ ⟫
+  | app  {Γ : Ctx Δ} {t₁ t₂ : Δ ⊢F⋆ ⋆} : Term Γ f⋆⟪ !t₁ → !t₂ ⟫ → Term Γ t₁ → Term Γ t₂
 
-  | Λ    {Γ : Ctx Δ} {k} {t : Δ ,⋆ k ⊢F⋆ ⋆} : Term (Γ ,,⋆ k) t → Term Γ ⋆⟪ ∀. !t ⟫
-  | sub  {Γ : Ctx Δ} {k} {t₁ : Δ ,⋆ k ⊢F⋆ ⋆} : Term Γ ⋆⟪ ∀. !t₁ ⟫ → (t₂ : Δ ⊢F⋆ k) → Term Γ (t₁[t₂]⋆)
+  | Λ    {Γ : Ctx Δ} {k} {t : Δ ,⋆ k ⊢F⋆ ⋆} : Term (Γ ,,⋆ k) t → Term Γ f⋆⟪ ∀. !t ⟫
+  | sub  {Γ : Ctx Δ} {k} {t₁ : Δ ,⋆ k ⊢F⋆ ⋆} : Term Γ f⋆⟪ ∀. !t₁ ⟫ → (t₂ : Δ ⊢F⋆ k) → Term Γ (t₁[t₂]⋆)
 
   | prim {Γ : Ctx Δ} : Term Γ .int → Prim → Term Γ .int → Term Γ .int
-  | pair {Γ : Ctx Δ} : Term Γ t₁ → Term Γ t₂ → Term Γ ⋆⟪ !t₁ × !t₂ ⟫
-  | fst  {Γ : Ctx Δ} : Term Γ ⋆⟪ !t₁ × !t₂ ⟫ → Term Γ t₁
-  | snd  {Γ : Ctx Δ} : Term Γ ⋆⟪ !t₁ × !t₂ ⟫ → Term Γ t₂
+  | pair {Γ : Ctx Δ} : Term Γ t₁ → Term Γ t₂ → Term Γ f⋆⟪ !t₁ × !t₂ ⟫
+  | fst  {Γ : Ctx Δ} : Term Γ f⋆⟪ !t₁ × !t₂ ⟫ → Term Γ t₁
+  | snd  {Γ : Ctx Δ} : Term Γ f⋆⟪ !t₁ × !t₂ ⟫ → Term Γ t₂
   | if0  {Γ : Ctx Δ} {t : Δ ⊢F⋆ ⋆} : Term Γ .int → Term Γ t → Term Γ t → Term Γ t
   deriving Repr
 
 namespace Term 
-  notation:50 Γ " ⊢ " t => Term Γ t
+  notation:50 Γ " ⊢F " t => Term Γ t
 
   syntax "get_elem'" (ppSpace term) : tactic
   macro_rules | `(tactic| get_elem' $n) => match n.1.toNat with
@@ -29,8 +29,8 @@ namespace Term
 
   macro "# " n:term:90 : term => `(Term.var (by get_elem' $n))
 
-  example : (∅ ,, ⋆⟪ int → int ⟫ ,, .int) ⊢ ⋆⟪ int ⟫ := #0
-  example : (∅ ,, ⋆⟪ int → int ⟫ ,, .int) ⊢ ⋆⟪ int → int ⟫ := #1
+  example : (∅ ,, f⋆⟪ int → int ⟫ ,, .int) ⊢F f⋆⟪ int ⟫ := #0
+  example : (∅ ,, f⋆⟪ int → int ⟫ ,, .int) ⊢F f⋆⟪ int → int ⟫ := #1
   
   declare_syntax_cat trm
   syntax "!" term:max : trm
@@ -50,39 +50,37 @@ namespace Term
   syntax "if0 " " ( " trm " , " trm " , " trm " ) " : trm
 
   syntax " ( " trm " ) " : trm
-  syntax " ⟪ " trm " ⟫" : term
+  syntax " f⟪ " trm " ⟫" : term
 
   macro_rules
-    | `( ⟪ !$t ⟫) => `($t)
-    | `( ⟪ $i:num ⟫ ) => `(Term.int $i)
-    | `( ⟪ #$i:num ⟫ ) => `(#$i)
-    | `( ⟪ λ. $e ⟫ ) => `(Term.fix ⟪ $e ⟫)
-    | `( ⟪ $e₁ $e₂  ⟫) => `(Term.app ⟪ $e₁ ⟫ ⟪ $e₂ ⟫ )
-    | `( ⟪ Λ. $e ⟫ ) => `(Term.Λ ⟪ $e ⟫ )
-    | `( ⟪ $e[$t] ⟫ ) => `(Term.sub ⟪ $e ⟫ ⋆⟪ $t ⟫)
-    | `( ⟪ $e₁ + $e₂ ⟫ ) => `(Term.prim ⟪ $e₁ ⟫ Prim.plus ⟪ $e₂ ⟫ )
-    | `( ⟪ $e₁ - $e₂ ⟫ ) => `(Term.prim ⟪ $e₁ ⟫ Prim.minus ⟪ $e₂ ⟫ )
-    | `( ⟪ $e₁ * $e₂ ⟫ ) => `(Term.prim ⟪ $e₁ ⟫ Prim.times ⟪$e₂ ⟫ )
-    | `( ⟪ ($e₁, $e₂) ⟫) => `(Term.pair ⟪ $e₁ ⟫ ⟪$e₂ ⟫ )
-    | `( ⟪ π₁ $e ⟫) => `(Term.fst ⟪ $e ⟫ )
-    | `( ⟪ π₂ $e ⟫) => `(Term.snd ⟪ $e ⟫ )
-    | `( ⟪ if0 $e₁ then $e₂ else $e₃ end ⟫ ) => `(Term.if0 ⟪ $e₁ ⟫ ⟪ $e₂ ⟫ ⟪ $e₃ ⟫ )
-    | `( ⟪ if0 ($e₁, $e₂, $e₃) ⟫ ) => `(Term.if0 ⟪ $e₁ ⟫ ⟪ $e₂ ⟫ ⟪ $e₃ ⟫ )
+    | `( f⟪ !$t ⟫) => `($t)
+    | `( f⟪ $i:num ⟫ ) => `(Term.int $i)
+    | `( f⟪ #$i:num ⟫ ) => `(#$i)
+    | `( f⟪ λ. $e ⟫ ) => `(Term.fix f⟪ $e ⟫)
+    | `( f⟪ $e₁ $e₂  ⟫) => `(Term.app f⟪ $e₁ ⟫ f⟪ $e₂ ⟫ )
+    | `( f⟪ Λ. $e ⟫ ) => `(Term.Λ f⟪ $e ⟫ )
+    | `( f⟪ $e[$t] ⟫ ) => `(Term.sub f⟪ $e ⟫ f⋆⟪ $t ⟫)
+    | `( f⟪ $e₁ + $e₂ ⟫ ) => `(Term.prim f⟪ $e₁ ⟫ Prim.plus f⟪ $e₂ ⟫ )
+    | `( f⟪ $e₁ - $e₂ ⟫ ) => `(Term.prim f⟪ $e₁ ⟫ Prim.minus f⟪ $e₂ ⟫ )
+    | `( f⟪ $e₁ * $e₂ ⟫ ) => `(Term.prim f⟪ $e₁ ⟫ Prim.times f⟪$e₂ ⟫ )
+    | `( f⟪ ($e₁, $e₂) ⟫) => `(Term.pair f⟪ $e₁ ⟫ f⟪$e₂ ⟫ )
+    | `( f⟪ π₁ $e ⟫) => `(Term.fst f⟪ $e ⟫ )
+    | `( f⟪ π₂ $e ⟫) => `(Term.snd f⟪ $e ⟫ )
+    | `( f⟪ if0 $e₁ then $e₂ else $e₃ end ⟫ ) => `(Term.if0 f⟪ $e₁ ⟫ f⟪ $e₂ ⟫ f⟪ $e₃ ⟫ )
+    | `( f⟪ if0 ($e₁, $e₂, $e₃) ⟫ ) => `(Term.if0 f⟪ $e₁ ⟫ f⟪ $e₂ ⟫ f⟪ $e₃ ⟫ )
 
-    | `( ⟪ ( $e ) ⟫ ) => `( ⟪ $e ⟫ ) 
-
-
+    | `( f⟪ ( $e ) ⟫ ) => `(f⟪ $e ⟫) 
 end Term
 open Term
 
 namespace Examples 
-  def fact :  ∅ ⊢ ⋆⟪ int → int ⟫ :=
+  def fact :  ∅ ⊢F f⋆⟪ int → int ⟫ :=
     Term.fix (.if0 (.var .here)
         (.int 1)
         (.prim (.var .here) .times (.app (.var (.there .here)) (Term.prim (.var .here) .minus (.int 1)))))
 
-  def fact' : ∅ ⊢ ⋆⟪ int → int ⟫ := 
-    ⟪ λ.
+  def fact' : ∅ ⊢F f⋆⟪ int → int ⟫ := 
+    f⟪ λ.
       if0 #0 then
         1
       else
@@ -91,19 +89,19 @@ namespace Examples
 
   theorem fact_eq_fact' : fact = fact' := rfl
 
-  def sixfact := ⟪ !fact 6 ⟫
+  def sixfact := f⟪ !fact 6 ⟫
 
-  def polyid : ∅ ⊢ ⋆⟪ ∀. ♯0 → ♯0 ⟫ :=  
-    ⟪ Λ. λ. #0 ⟫
+  def polyid : ∅ ⊢F f⋆⟪ ∀. ♯0 → ♯0 ⟫ :=  
+    f⟪ Λ. λ. #0 ⟫
 
-  def intid : ∅ ⊢ ⋆⟪ int → int ⟫ :=
-    ⟪ (!polyid)[int] ⟫
+  def intid : ∅ ⊢F f⋆⟪ int → int ⟫ :=
+    f⟪ (!polyid)[int] ⟫
 
-  def twice : ∅ ⊢ ⋆⟪ ∀. (♯0 → ♯0) → ♯0 → ♯0 ⟫ := 
-    ⟪ Λ. λ. #1 #1 #0 ⟫ 
+  def twice : ∅ ⊢F f⋆⟪ ∀. (♯0 → ♯0) → ♯0 → ♯0 ⟫ := 
+    f⟪ Λ. λ. #1 #1 #0 ⟫ 
 end Examples
 
-def conv_ent {Δ Γ} {t₁ t₂ : Δ ⊢F⋆ ⋆} : t₁ = t₂ → (Γ ⊢ t₁) → Γ ⊢ t₂
+def conv_ent {Δ Γ} {t₁ t₂ : Δ ⊢F⋆ ⋆} : t₁ = t₂ → (Γ ⊢F t₁) → Γ ⊢F t₂
   | rfl, a => a
 
 def Ren {Δ₁ Δ₂} (Γ₁ : Ctx Δ₁) (Γ₂ : Ctx Δ₂) : Renτ Δ₁ Δ₂ → Type := 
@@ -127,7 +125,7 @@ def τlift {Δ₁ Δ₂ Γ₁ Γ₂} {rt : Renτ Δ₁ Δ₂} (r : Ren Γ₁ Γ�
 
 
 def ren {Δ₁ Δ₂ Γ₁ Γ₂} {rt : Renτ Δ₁ Δ₂} (r : Ren Γ₁ Γ₂ rt) :
-  {t : Δ₁ ⊢F⋆ ⋆} → (Γ₁ ⊢ t) → (Γ₂ ⊢ renτ rt t)
+  {t : Δ₁ ⊢F⋆ ⋆} → (Γ₁ ⊢F t) → (Γ₂ ⊢F renτ rt t)
   | _, .int i => .int i
   | _, .var x => .var (r x)
 
@@ -146,16 +144,16 @@ def ren {Δ₁ Δ₂ Γ₁ Γ₂} {rt : Renτ Δ₁ Δ₂} (r : Ren Γ₁ Γ₂ 
   | _, .snd e => .snd (ren r e)
   | _, .if0 e₁ e₂ e₃ => .if0 (ren r e₁) (ren r e₂) (ren r e₃)
 
-def weaken {Δ Γ} {t₁ t₂ : Δ ⊢F⋆ ⋆} (e : Γ ⊢ t₁) : (Γ ,, t₂ ⊢ t₁) := by
+def weaken {Δ Γ} {t₁ t₂ : Δ ⊢F⋆ ⋆} (e : Γ ⊢F t₁) : (Γ ,, t₂ ⊢F t₁) := by
   apply conv_ent; rotate_left 1
   · exact (ren (conv_ni (Eq.symm renτ_id) ∘ .there) e)
   · apply renτ_id
 
-def tweaken {Δ Γ} (t : Δ ⊢F⋆ ⋆) {k} (e : Γ ⊢ t) : Γ ,,⋆ k ⊢ weakenτ t :=
+def tweaken {Δ Γ} (t : Δ ⊢F⋆ ⋆) {k} (e : Γ ⊢F t) : Γ ,,⋆ k ⊢F weakenτ t :=
   ren .move e
 
 def Subs {Δ₁ Δ₂} (Γ₁ : Ctx Δ₁) (Γ₂ : Ctx Δ₂) (st : Subsτ Δ₁ Δ₂) : Type := 
-  {t : Δ₁ ⊢F⋆ ⋆} → (Γ₁ ∋ t) → (Γ₂ ⊢ subsτ st t)
+  {t : Δ₁ ⊢F⋆ ⋆} → (Γ₁ ∋ t) → (Γ₂ ⊢F subsτ st t)
 
 def lifts {Δ₁ Δ₂ Γ₁ Γ₂} (st : Subsτ Δ₁ Δ₂) (s : Subs Γ₁ Γ₂ st) {t : Δ₁ ⊢F⋆ ⋆} : Subs (Γ₁ ,, t) (Γ₂ ,, subsτ st t) st
   | _, .here => .var .here
@@ -173,7 +171,7 @@ def tlifts {Δ₁ Δ₂ Γ₁ Γ₂} (st : Subsτ Δ₁ Δ₂) (s : Subs Γ₁ �
       congr
 
 def subs {Δ₁ Δ₂ Γ₁ Γ₂} (st : Subsτ Δ₁ Δ₂) (s : Subs Γ₁ Γ₂ st) 
-  {t : Δ₁ ⊢F⋆ ⋆} : (Γ₁ ⊢ t) → (Γ₂ ⊢ subsτ st t)
+  {t : Δ₁ ⊢F⋆ ⋆} : (Γ₁ ⊢F t) → (Γ₂ ⊢F subsτ st t)
   | .int i => .int i
   | .var x => s x
 
@@ -197,23 +195,23 @@ def subs {Δ₁ Δ₂ Γ₁ Γ₂} (st : Subsτ Δ₁ Δ₂) (s : Subs Γ₁ Γ�
   | .snd e => .snd (subs st s e)
   | .if0 e₁ e₂ e₃ => .if0 (subs st s e₁) (subs st s e₂) (subs st s e₃)
 
-def extend {Δ₁ Δ₂ Γ₁ Γ₂} (st : Subsτ Δ₁ Δ₂) (s : Subs Γ₁ Γ₂ st) {t : Δ₁ ⊢F⋆ ⋆} : (Γ₂ ⊢ subsτ st t) → Subs (Γ₁ ,, t) Γ₂ st 
+def extend {Δ₁ Δ₂ Γ₁ Γ₂} (st : Subsτ Δ₁ Δ₂) (s : Subs Γ₁ Γ₂ st) {t : Δ₁ ⊢F⋆ ⋆} : (Γ₂ ⊢F subsτ st t) → Subs (Γ₁ ,, t) Γ₂ st 
   | e, _, .here => e
   | _, _, .there x => s x
 
-def subs_extend {Δ Γ k} {t₁ : Δ ,⋆ k ⊢F⋆ ⋆} {t₂ : Δ ⊢F⋆ k} (x : Γ ,,⋆ k ∋ t₁): Γ ⊢ subsτ (extendτ .var t₂) t₁ := by
+def subs_extend {Δ Γ k} {t₁ : Δ ,⋆ k ⊢F⋆ ⋆} {t₂ : Δ ⊢F⋆ k} (x : Γ ,,⋆ k ∋ t₁): Γ ⊢F subsτ (extendτ .var t₂) t₁ := by
   cases x
   rename_i x
   apply conv_ent; rotate_left 1
   · exact (.var x)
   · simp [weakenτ]
     rw [←subsτ_renτ]
-    have : (fun {j} => extendτ (fun {j} => Typ.var) t₂ ∘ Lookupt.there) = fun {j} => @Typ.var Δ j := by
+    have : (fun {j} => extendτ (fun {j} => TypF.var) t₂ ∘ Lookupt.there) = fun {j} => @TypF.var Δ j := by
       funext j x
       cases x <;> rfl
     rw [this, subsτ_id]
 
-def subs_one {Δ Γ} {t₁ t₂ : Δ ⊢F⋆ ⋆} : (Γ ,, t₂ ⊢ t₁) → (Γ ⊢ t₂) → (Γ ⊢ t₁) := by
+def subs_one {Δ Γ} {t₁ t₂ : Δ ⊢F⋆ ⋆} : (Γ ,, t₂ ⊢F t₁) → (Γ ⊢F t₂) → (Γ ⊢F t₁) := by
   intro e₂ e₁
   apply conv_ent; rotate_left 1
   · exact (subs .var
@@ -226,13 +224,13 @@ def subs_one {Δ Γ} {t₁ t₂ : Δ ⊢F⋆ ⋆} : (Γ ,, t₂ ⊢ t₁) → (�
 macro b:term:80 ".[" a:term:80 "]" : term =>
   `(subs_one $b $a)
 
-def tsubs_one {Δ Γ k} {t₁ : Δ ,⋆ k ⊢F⋆ ⋆} (e : Γ ,,⋆ k ⊢ t₁) (t₂ : Δ ⊢F⋆ k) : Γ ⊢ (t₁[t₂]⋆) := subs (extendτ .var t₂) subs_extend e
+def tsubs_one {Δ Γ k} {t₁ : Δ ,⋆ k ⊢F⋆ ⋆} (e : Γ ,,⋆ k ⊢F t₁) (t₂ : Δ ⊢F⋆ k) : Γ ⊢F (t₁[t₂]⋆) := subs (extendτ .var t₂) subs_extend e
 
 macro b:term:80 "⋆[" a:term:80 "]" : term =>
   `(tsubs_one $b $a)
 
-example : (⟪ #0 ⟫.[⟪ (1, 2) ⟫] : ∅ ⊢ ⋆⟪ int × int ⟫) =
-           ⟪ (1, 2) ⟫                               := rfl
+example : (f⟪ #0 ⟫.[f⟪ (1, 2) ⟫] : ∅ ⊢F f⋆⟪ int × int ⟫) =
+           f⟪ (1, 2) ⟫                                  := rfl
 
-example : (⟪ λ. #1 #0 ⟫.[⟪ (6, 9) ⟫] : ∅  ⊢ ⋆⟪ int → int ⟫) =
-           ⟪ λ. #1 #0 ⟫                                    := rfl
+example : (f⟪ λ. #1 #0 ⟫.[f⟪ (6, 9) ⟫] : ∅ ⊢F f⋆⟪ int → int ⟫) =
+           f⟪ λ. #1 #0 ⟫                                      := rfl
