TypedAssembly/LambdaF/Step.lean
@@ -1,12 +1,12 @@
 import «TypedAssembly».LambdaF.Term
 
-inductive Value : {Δ : Ctxt} → {Γ : Ctx Δ} → {t : Δ ⊢F⋆ ⋆} → (Γ ⊢ t) → Prop where
-  | v_int : Value (.int i)
-  | v_fix : Value (.fix e)
-  | v_Λ  : Value e → Value (.Λ e)
+inductive Value : {Γ : Ctx Δ} → {t : Δ ⊢F⋆ ⋆} → (Γ ⊢F t) → Prop where
+  | v_int  : Value (.int i)
+  | v_fix  : Value (.fix e)
+  | v_Λ    : Value e → Value (.Λ e)
   | v_pair : Value e₁ → Value e₂ → Value (.pair e₁ e₂)
 
-inductive Step : {Δ : Ctxt} → {Γ : Ctx Δ} → {t : Δ ⊢F⋆ ⋆} → (Γ ⊢ t) → (Γ ⊢ t) → Prop
+inductive Step : {Δ : Ctxt} → {Γ : Ctx Δ} → {t : Δ ⊢F⋆ ⋆} → (Γ ⊢F t) → (Γ ⊢F t) → Prop
   | app_exec   : Value a → Step (.app (.fix e) a) (e.[weaken a].[.fix e])
   | app_right  : Value a → Step b b' → Step (.app a b) (.app a b')
   | app_left   : Step a a' → Step (.app a e) (.app a' e)
@@ -20,25 +20,25 @@ inductive Step : {Δ : Ctxt} → {Γ : Ctx Δ} → {t : Δ ⊢F⋆ ⋆} → (Γ 
   | prim_right : Step b b' → Step (.prim (.int n) p b) (.prim (.int n) p b')
   | prim_left  : Step a a' → Step (.prim a p b) (.prim a' p b)
   
-  | pair_left  : Step a a' → Step ⟪ (!a, !b) ⟫ ⟪ (!a', !b) ⟫
-  | pair_right : Value a → Step b b' → Step ⟪ (!a, !b) ⟫ ⟪ (!a, !b') ⟫
+  | pair_left  : Step a a' → Step f⟪ (!a, !b) ⟫ f⟪ (!a', !b) ⟫
+  | pair_right : Value a → Step b b' → Step f⟪ (!a, !b) ⟫ f⟪ (!a, !b') ⟫
 
-  | fst_exec   : Step ⟪ π₁(!e, !e') ⟫ e
+  | fst_exec   : Step f⟪ π₁(!e, !e') ⟫ e
   | fst_steps  : Step e e' →  Step (.fst e) (.fst e')
 
-  | snd_exec   : Step ⟪ π₂(!e', !e) ⟫ e
+  | snd_exec   : Step f⟪ π₂(!e', !e) ⟫ e
   | snd_steps  : Step e e' →  Step (.snd e) (.snd e')
 
-  | if0_exec   : Step ⟪ if0 0 then !b else !c end ⟫ b
-  | ifn0_exec  : n ≠ 0 → Step ⟪ if0 !(.int n) then !b else !c end ⟫ c
-  | if_steps   : Step a a' → Step ⟪ if0 !a then !b else !c end ⟫ ⟪ if0 !a' then !b else !c end ⟫
+  | if0_exec   : Step f⟪ if0 0 then !b else !c end ⟫ b
+  | ifn0_exec  : n ≠ 0 → Step f⟪ if0 !(.int n) then !b else !c end ⟫ c
+  | if_steps   : Step a a' → Step f⟪ if0 !a then !b else !c end ⟫ f⟪ if0 !a' then !b else !c end ⟫
 
 namespace Step 
   infixr:90 " ==> " => Step
 end Step
 open Step
 
-inductive MultiStep {Δ} {Γ : Ctx Δ} {t : Δ ⊢F⋆ ⋆} : (Γ ⊢ t) → (Γ ⊢ t) → Prop 
+inductive MultiStep {Δ} {Γ : Ctx Δ} {t : Δ ⊢F⋆ ⋆} : (Γ ⊢F t) → (Γ ⊢F t) → Prop 
   | refl {a} : MultiStep a a
   | step {a b c} : a ==> b → MultiStep b c → MultiStep a c
 
@@ -47,27 +47,20 @@ namespace MultiStep
 end MultiStep
 open MultiStep
 
-example : ⟪ if0 0 then 1 + 1 * 1 else 5 * 1 end ⟫ ==>* (⟪ 2 ⟫ : ∅ ⊢ .int) := by
+example : f⟪ if0 0 then 1 + 1 * 1 else 5 * 1 end ⟫ ==>* (f⟪ 2 ⟫ : ∅ ⊢F .int) := by
   repeat constructor
 
-example : ⟪ if0 1 then 1 + 1 * 1 else 5 * 1 end ⟫ ==>* (⟪ 5 ⟫ : ∅ ⊢ .int) := by
+example : f⟪ if0 1 then 1 + 1 * 1 else 5 * 1 end ⟫ ==>* (f⟪ 5 ⟫ : ∅ ⊢F .int) := by
   repeat constructor
   · intros contra; contradiction
   · repeat constructor
 
 open Examples in
-example : ⟪ !fact 0 ⟫ ==>* ⟪ 1 ⟫ := by
-  unfold fact
-  apply MultiStep.step
-  · apply Step.app_exec
-    constructor
-  · apply MultiStep.step
-    · simp [subs_one, conv_ent, subs]
-      apply Step.if0_exec
-    · apply MultiStep.refl
+example : f⟪ !fact 0 ⟫ ==>* f⟪ 1 ⟫ := by
+  repeat constructor
 
 open Examples in
-example : ⟪ !fact 3 ⟫ ==>* ⟪ 6 ⟫ := by
+example : f⟪ !fact 3 ⟫ ==>* f⟪ 6 ⟫ := by
   unfold fact
   apply MultiStep.step
   · apply Step.app_exec
@@ -128,7 +121,7 @@ example : ⟪ !fact 3 ⟫ ==>* ⟪ 6 ⟫ := by
                       repeat constructor <;> repeat constructor
 
 open Examples in
-example : ⟪ !intid 6 ⟫ ==>* ⟪ 6 ⟫ := by
+example : f⟪ !intid 6 ⟫ ==>* f⟪ 6 ⟫ := by
   unfold intid
   constructor
   · apply Step.app_left
